Clap/eDSLState/WitnessGenerator/eq0.lean
@@ -7,6 +7,22 @@ namespace WitnessGenerator
 def eq0 {p : ℕ} (_cache : ValueCache p) (trace : Array (ZMod p)) (_expr : ExprRef) : Array (ZMod p) :=
   trace
 
+namespace eq0
+
+def trace_capacity : ℕ := 0
+
+@[simp, grind =]
+lemma trace_size_eq
+  {p}
+  (cache : ValueCache p)
+  (trace : Array (ZMod p))
+  (expr : ExprRef)
+:
+  (eq0 cache trace expr).size = trace.size + trace_capacity
+:= rfl
+
+end eq0
+
 end WitnessGenerator
 
 end Clap
