Clap/eDSLState/WitnessGenerator/fpMul.lean
@@ -1,117 +1,378 @@
 import Clap.eDSLState.Expr
+import Clap.eDSLState.HashCons.Eval
 import Clap.eDSLState.WitnessGenerator.isZero
 import Clap.eDSLState.WitnessGenerator.num2bits
 
 import CompPoly.Univariate.Basic
 
-namespace Clap
+namespace Clap.WitnessGenerator
 
-section Andrew
+section FpMulImplementation
 
-open CompPoly
+open CompPoly HashConsM
 
 variable {p : ℕ} {var : Type} [inst : Fact (Nat.Prime p)] [inst' : Fact (p > 2)]
-
-namespace WitnessGenerator
 
 def toCompPoly {k : ℕ} (vec : Vector (ZMod p) k) : CPolynomial (ZMod p) :=
   List.foldr (fun i p ↦ p + CPolynomial.C (vec[i]) * CPolynomial.X ^ i.1) 0 (List.finRange k)
 
 def rangeCheckVec
-  (cache : ValueCache p) (trace : Array (ZMod p)) {w : ℕ} (vec : Vector ExprRef w) : Array (ZMod p) :=
-  vec.foldr (fun e trace ↦ num2bits cache trace w e) trace
+  {k}
+  (cache : ValueCache p) (trace : Array (ZMod p))
+  (width : ℕ) (vec : Vector ExprRef k)
+: Array (ZMod p) :=
+  vec.foldr (fun e trace ↦ num2bitsUnsafe cache trace width e) trace
+
+def rangeCheckInputs
+  {k}
+  (cache : ValueCache p)
+  (trace : Array (ZMod p))
+  (width : ℕ)
+  (a b p' : Vector ExprRef k)
+: Array (ZMod p) :=
+  let trace := rangeCheckVec cache trace width a
+  let trace := rangeCheckVec cache trace width b
+  let trace := rangeCheckVec cache trace width p'
+  trace
 
 def carry (w : ℕ) : List (ZMod p) → ZMod p → List (ZMod p)
 | l :: l' :: ls, c => let c' : ZMod p := (l + c) / (2 ^ w); c' :: carry w (l' :: ls) c'
 | _ :: []      , _ => []
 | []           , _ => []
 
-def checkCarryZero {k : ℕ}
-  (cache : ValueCache p) (trace : Array (ZMod p)) (w : ℕ) (t : Vector ExprRef k) : HashConsM p (Array (ZMod p)) := do
+def insertListInCache
+  (cache : ValueCache p) (trace : Array (ZMod p))
+  (l : List (ZMod p))
+:
+  HashConsM p (ValueCache p × List (BoundRef p))
+:= do
+  let refs ← l.mapM .mkConstant
+  let varStore := (Std.ExtTreeMap.ofArray (trace.zipIdx.map Prod.swap))
+  let σ ← get
+  let cache := refs.foldr (λ ref cache => Expr.evalWithCache varStore cache ⦃ref, σ⦄) cache
+  return (cache, refs)
+
+def insertVecInCache
+  {k}
+  (cache : ValueCache p) (trace : Array (ZMod p))
+  (vec : Vector (ZMod p) k)
+:
+  HashConsM p (ValueCache p × Vector (BoundRef p) k)
+:= do
+  let refs ← vec.mapM .mkConstant
+  let varStore := (Std.ExtTreeMap.ofArray (trace.zipIdx.map Prod.swap))
+  let σ ← get
+  let cache := refs.foldr (λ ref cache => Expr.evalWithCache varStore cache ⦃ref, σ⦄) cache
+  return (cache, refs)
+
+def checkCarryZeroUnsafe {k : ℕ}
+  (cache : ValueCache p) (trace : Array (ZMod p)) (w : ℕ) (t : Vector ExprRef k)
+: HashConsM p (Array (ZMod p)) := do
   let carry : List (ZMod p) := carry w (t.toList.map (cache[·]!.get!)) 0
   let trace := trace ++ carry
-  let num2bits ←
-    carry.foldrM (init := trace) fun c trace ↦ do
-      return num2bits cache trace (w + Nat.clog 2 k + 2) (←.mkConstant (c + (2 ^ (w + 1) * k)))
-  return trace ++ num2bits
+  let (cache, carry_constants) ← insertListInCache cache trace (carry.map (· + (2 ^ (w + 1) * k)))
+  return carry_constants.foldr (init := trace) fun c trace ↦
+    num2bitsUnsafe cache trace (w + Nat.clog 2 k + 2) c
+
+
+def mkOr {p} (a b : BoundRef p) : HashConsM p (BoundRef p) := do
+  (←a + b) - (←a*b)
+
+def mkNot {p} (a : BoundRef p) : HashConsM p (BoundRef p) := do
+  (←mkConstant 1) - a
 
 def check_lt_wg' {k : ℕ}
-  (cache : ValueCache p) (trace : Array (ZMod p)) (w : ℕ) (isLt : HashConsM.BoundRef p)
-  (t₀ : Vector (HashConsM.BoundRef p) k) (t₁ : Vector (HashConsM.BoundRef p) k) : HashConsM p (Array (ZMod p)) :=
+  (cache : ValueCache p) (trace : Array (ZMod p)) (w : ℕ)
+  (isLt : HashConsM.BoundRef p)
+  (t₀ : Vector (HashConsM.BoundRef p) k) (t₁ : Vector (HashConsM.BoundRef p) k)
+: HashConsM p (ValueCache p × Array (ZMod p)) :=
   match k with
-  | .zero => return trace
+  | .zero => return (cache, trace)
   | .succ k => do
     let tδ ← t₀[Fin.last k] - t₁[Fin.last k]
-    let num2bits_trace := num2bits cache trace w
-      (←(←(←.mkConstant 1) - isLt) *
-        (←(tδ + (←.mkConstant ((2 ^ w : ZMod p) - 1))))
-      )
-    let trace := trace ++ num2bits_trace
-    let isZero_trace := isZero cache trace tδ
-    let trace := trace ++ isZero_trace
-    
-    -- (fun _ ↦
-    --   IsZero.isZero_wg (t₀[Fin.last k] - t₁[Fin.last k])
-    --     (fun iz ↦
-    --       let isLt' : Expₑ p :=
-    --         isLt ||| (1 - .v iz)
-    --       check_lt_wg' w isLt' (Vector.ofFn (fun i ↦ t₀[(i.castSucc)])) (Vector.ofFn (fun i ↦ t₁[(i.castSucc)])) cont
-    --     )
-    -- )
-    _
+    let x ←(←(←.mkConstant 1) - isLt) * (←(tδ + (←.mkConstant ((2 ^ w : ZMod p) - 1))))
+    let varStore := (Std.ExtTreeMap.ofArray (trace.zipIdx.map Prod.swap))
+    let cache := Expr.evalWithCache varStore cache ⦃x, ←get⦄
+    let trace := num2bitsUnsafe cache trace w x
 
-def checkLt {k : ℕ} (w : ℕ) (t : Vector (Expₑ p) k) (t' : Vector (Expₑ p) k) (cont : Wg p) : Wg p :=
-  check_lt_wg' w 0 t t' cont
+    -- The cache must contain tδ because it is a subexpression of x
+    let trace := isZeroUnsafe cache trace tδ
+    let isZero := trace.back!
 
-def fpMul {k : ℕ}
+    let isLt' ← mkOr isLt (←(←mkConstant 1) - (←mkConstant isZero))
+
+    let varStore := (Std.ExtTreeMap.ofArray (trace.zipIdx.map Prod.swap))
+    let cache := Expr.evalWithCache varStore cache ⦃isLt', ←get⦄
+
+    check_lt_wg' cache trace w isLt' (Vector.ofFn (fun i ↦ t₀[(i.castSucc)])) (Vector.ofFn (fun i ↦ t₁[(i.castSucc)]))
+
+
+def checkLtUnsafe {k : ℕ}
   (cache : ValueCache p) (trace : Array (ZMod p))
-  (w : ℕ) (a b p' : Vector ExprRef k) : HashConsM p (Array (ZMod p)) := do
-  let rangeCheckeda := rangeCheckVec cache trace a
-  let rangeCheckedb := rangeCheckVec cache trace b
-  let rangeCheckedp' := rangeCheckVec cache trace p'
-  let trace := trace ++ rangeCheckeda ++ rangeCheckedb ++ rangeCheckedp'
+  (w : ℕ) (t₀ : Vector (HashConsM.BoundRef p) k) (t₁ : Vector (HashConsM.BoundRef p) k)
+: HashConsM p (ValueCache p × Array (ZMod p)) := do
+  check_lt_wg' cache trace w (←mkConstant 0) t₀ t₁
 
+
+def polyMult
+  {k}
+  (cache : ValueCache p) (trace : Array (ZMod p))
+  (a b : Vector ExprRef k)
+: CPolynomial (ZMod p) × Array (ZMod p) :=
   let ab := toCompPoly (a.map (cache[·]!.get!)) * toCompPoly (b.map (cache[·]!.get!))
   let ab_trace := Array.range (2 * k -1) |>.map ab.coeff
-  let trace := trace ++ ab_trace
+  (ab, trace ++ ab_trace)
 
-  let a_val : ℕ := ∑ i : Fin k, cache[a[i]]!.get!.val * (2 ^ w) ^ i.1
-  let b_val : ℕ := ∑ i : Fin k, cache[b[i]]!.get!.val * (2 ^ w) ^ i.1
-  let p_val : ℕ := ∑ i : Fin k, cache[p'[i]]!.get!.val * (2 ^ w) ^ i.1
+def allocUncheckedUnsafe
+  {k : ℕ}
+  (cache : ValueCache p) (trace : Array (ZMod p))
+  (values : Vector ExprRef k)
+: Array (ZMod p) :=
+  trace ++ values.toArray.map (cache[·]!.get!)
+
+def allocRangeCheckedUnsafe
+  {k : ℕ}
+  (cache : ValueCache p) (trace : Array (ZMod p))
+  (width : ℕ)
+  (values : Vector ExprRef k)
+: Array (ZMod p) :=
+  let trace := allocUncheckedUnsafe cache trace values
+  rangeCheckVec cache trace width values
+
+
+def fpMulUnsafe {k : ℕ}
+  (cache : ValueCache p) (trace : Array (ZMod p))
+  (width : ℕ) (a b p' : Vector ExprRef k)
+: HashConsM p (ValueCache p × Array (ZMod p)) := do
+  let trace := rangeCheckInputs cache trace width a b p'
+
+  let (ab, trace) := polyMult cache trace a b
+
+  let a_val : ℕ := ∑ i : Fin k, cache[a[i]]!.get!.val * (2 ^ width) ^ i.1
+  let b_val : ℕ := ∑ i : Fin k, cache[b[i]]!.get!.val * (2 ^ width) ^ i.1
+  let p_val : ℕ := ∑ i : Fin k, cache[p'[i]]!.get!.val * (2 ^ width) ^ i.1
   let q_val : ℕ := (a_val * b_val) / p_val
   let r_val : ℕ := (a_val * b_val) % p_val
 
-  let q_vec := natToLimbsV (p := p) w k q_val
-  let trace := trace ++ q_vec.toArray
+  let q_vec := natToLimbsV (p := p) width k q_val
+  let (cache, q_vec_constants) ← insertVecInCache cache trace q_vec
+  let trace := allocRangeCheckedUnsafe cache trace width q_vec_constants
 
-  let q_vec_constants ← q_vec.mapM .mkConstant
-  let rangeCheckedq_vec_constants := rangeCheckVec cache trace q_vec_constants
-  let trace := trace ++ rangeCheckedq_vec_constants
-
-  let r_vec := natToLimbsV (p := p) w k r_val
-  let trace := trace ++ r_vec.toArray
-
-  let r_vec_constants ← r_vec.mapM .mkConstant
-  let rangeCheckedr_vec_constants := rangeCheckVec cache trace r_vec_constants
-  let trace := trace ++ rangeCheckedq_vec_constants
+  let r_vec := natToLimbsV (p := p) width k r_val
+  let (cache, r_vec_constants) ← insertVecInCache cache trace r_vec
+  let trace := allocRangeCheckedUnsafe cache trace width r_vec_constants
 
   let t := ab - toCompPoly (p'.map (cache[·]!.get!)) * toCompPoly q_vec - toCompPoly r_vec
-  let t_trace := List.range (2 * k - 1) |>.map t.coeff
-  let trace := trace ++ t_trace
+  let (cache, t_vec_constants) ← insertVecInCache cache trace (Vector.range (2 * k - 1) |>.map t.coeff)
+  let trace := allocUncheckedUnsafe cache trace t_vec_constants
 
-  let checkCarryZero :=
-    checkCarryZero cache trace w
-      (←Vector.ofFnM (fun i : Fin (2 * k - 1) ↦ .mkConstant (t.coeff i.1)))
-  
-  check_lt_wg w (r_vec.map .c) p'
-  _
-  -- let ws :=
-  --   (List.finRange (2 * k - 1)).foldr
-  --     (fun i (trace : Array (ZMod p)) ↦ trace.push (ab.coeff i)) <|
-  --     q_vec.foldr (flip Array.push) <|
+  let trace ← checkCarryZeroUnsafe cache trace width t_vec_constants
 
-end WitnessGenerator
+  checkLtUnsafe cache trace width r_vec_constants p'
 
-end Andrew
+end FpMulImplementation
 
-end Clap
+namespace fpMul
+
+def trace_capacity (k width: ℕ) : ℕ :=
+  3 * k * num2bits.trace_capacity width +
+  (2 * k - 1) + k * (num2bits.trace_capacity width + 1) +
+  k * (num2bits.trace_capacity width + 1) +
+  (2 * k - 1) +
+  (2 * k - 1 - 1) +
+  (2 * k - 1 - 1) * num2bits.trace_capacity (width + Nat.clog 2 (2 * k - 1) + 2) +
+  k * (num2bits.trace_capacity width + isZero.trace_capacity)
+
+@[simp, grind =]
+lemma rangeCheckVec_trace_size
+  {p} {k}
+  {cache : ValueCache p}
+  {trace : Array (ZMod p)}
+  {width}
+  {vec : Vector ExprRef k}
+:
+  (rangeCheckVec cache trace width vec).size = trace.size + k*num2bits.trace_capacity width
+:= by
+  simp [rangeCheckVec]
+  induction' k with k ih generalizing trace
+  . have : vec = #v[] := by grind
+    simp [this]
+  . have := Vector.push_pop_back vec
+    rewrite [←this]
+    simp
+    rewrite [ih]
+    grind
+
+@[simp, grind =]
+lemma rangeCheckInputs_trace_size
+  {p} {k}
+  {cache : ValueCache p}
+  {trace : Array (ZMod p)}
+  {width}
+  {a b p' : Vector ExprRef k}
+:
+  (rangeCheckInputs cache trace width a b p').size = trace.size + 3*k*num2bits.trace_capacity width
+:= by
+  grind [rangeCheckInputs]
+
+@[simp, grind=]
+lemma allocUncheckedUnsafe_trace_size
+  {p} {k}
+  {cache : ValueCache p}
+  {trace : Array (ZMod p)}
+  {values : Vector ExprRef k}
+:
+  (allocUncheckedUnsafe cache trace values).size = trace.size + k
+:= by
+  grind [allocUncheckedUnsafe]
+
+@[simp, grind=]
+lemma allocRangeCheckedUnsafe_trace_size
+  {p} {k}
+  {cache : ValueCache p}
+  {trace : Array (ZMod p)}
+  {width}
+  {values : Vector ExprRef k}
+:
+  (allocRangeCheckedUnsafe cache trace width values).size = trace.size + k*(num2bits.trace_capacity width + 1)
+:= by
+  grind [allocRangeCheckedUnsafe]
+
+@[simp, grind =]
+lemma carry_length
+  {p} [Fact p.Prime]
+  {width : ℕ}
+  {l : List (ZMod p)}
+  {c : ZMod p}
+:
+  (carry width l c).length = l.length - 1
+:= by
+  fun_induction carry
+  . grind
+  . grind
+  . grind
+
+@[simp, grind =]
+lemma insertListInCache_length
+  {p}
+  {cache : ValueCache p}
+  {trace : Array (ZMod p)}
+  {list : List (ZMod p)}
+  {σ}
+:
+  ((insertListInCache cache trace list).run σ).1.2.length =
+  list.length
+:= by
+  simp [insertListInCache]
+  induction' list with head tail ih generalizing σ cache trace
+  . rfl
+  . simp_rw [
+      ←HashConsM.getHashConsState.eq_def,
+      ←HashConsM.getResult.eq_def,
+    ] at ⊢ ih
+    simp
+
+@[simp, grind =]
+lemma checkCarryZeroUnsafe_trace_size
+  {p} [Fact p.Prime] {k}
+  {cache : ValueCache p}
+  {trace : Array (ZMod p)}
+  {width}
+  {t : Vector ExprRef k}
+  {σ}
+:
+  ((checkCarryZeroUnsafe cache trace width t).run σ).1.size =
+  trace.size +
+    (k-1) +
+    (k-1) * (
+      num2bits.trace_capacity (width + Nat.clog 2 k + 2)
+    )
+:= by
+  simp [
+    checkCarryZeroUnsafe,
+    ←HashConsM.getResult.eq_def
+  ]
+
+  set carry := carry width (List.map (fun x => cache[x]!.get!) t.toList) (0 : ZMod p)
+  have h_carry_length : carry.length = k-1 := by
+    grind
+  clear_value carry
+
+  obtain ⟨trace⟩ := trace
+  simp
+
+  set cache' := ((insertListInCache _ _ _).getResult σ).1
+  set carry_constants := ((insertListInCache _ _ _).getResult σ).2
+  have h_carry_constants : carry_constants.length = k - 1 :=  by
+    subst carry_constants
+    simp [HashConsM.getResult, insertListInCache_length, h_carry_length]
+  clear_value cache'
+  clear_value carry_constants
+
+  obtain _ | ⟨k⟩ := k
+  . grind
+  . simp at *
+    have : trace.length + k = (trace ++ carry).toArray.size := by grind
+    rewrite [this]
+    set width' := width + Nat.clog _ _ + 2
+    clear_value width'
+    rewrite [←h_carry_constants]
+    clear this h_carry_constants h_carry_length
+    induction carry_constants
+    . grind
+    . grind
+
+@[simp, grind =]
+lemma checkLtUnsafe_trace_size
+  {p} [Fact p.Prime] {k}
+  {cache : ValueCache p}
+  {trace : Array (ZMod p)}
+  {width}
+  {t1 t2 : Vector ExprRef k}
+  {σ}
+:
+  ((checkLtUnsafe cache trace width t1 t2).run σ).1.2.size =
+  trace.size + k*(num2bits.trace_capacity width + isZero.trace_capacity)
+:= by
+  simp [checkLtUnsafe, ←HashConsM.getResult.eq_def]
+  set x := if CacheExpr.c 0 ∈ σ.exprs then _ else _
+  set isLt := x.1
+  set σ := x.2
+  clear_value x
+  clear_value isLt
+  clear_value σ
+  induction' k with k ih generalizing cache trace width isLt σ
+  . unfold check_lt_wg'
+    grind
+  . unfold check_lt_wg'
+    simp
+    rewrite [ih]
+    grind
+
+@[simp, grind =]
+lemma polyMult_size
+  {p} [Fact p.Prime] {k}
+  {cache : ValueCache p}
+  {trace : Array (ZMod p)}
+  {a b : Vector ExprRef k}
+:
+  (polyMult cache trace a b).2.size =
+  trace.size + (2*k - 1)
+:= by
+  simp [polyMult]
+
+@[simp, grind =]
+lemma trace_size_eq
+  {p} [Fact p.Prime] {k}
+  {cache : ValueCache p}
+  {trace : Array (ZMod p)}
+  {width : ℕ}
+  (a b p' : Vector ExprRef k)
+  {σ}
+:
+  ((fpMulUnsafe cache trace width a b p').run σ).1.2.size = trace.size + trace_capacity k width
+:= by
+  simp [fpMulUnsafe, trace_capacity]
+  grind
+
+end Clap.WitnessGenerator.fpMul
