Clap/eDSLState/WitnessGenerator/share.lean
@@ -7,6 +7,23 @@ namespace WitnessGenerator
 def share {p : ℕ} (cache : ValueCache p) (trace : Array (ZMod p)) (expr : ExprRef): Array (ZMod p) :=
   trace.push cache[expr]!.get!
 
+namespace share
+
+def trace_capacity : ℕ := 1
+
+@[simp, grind =]
+lemma trace_size_eq
+  {p}
+  (cache : ValueCache p)
+  (trace : Array (ZMod p))
+  (expr : ExprRef)
+:
+  (share cache trace expr).size = trace.size + trace_capacity
+:= by
+  simp [share, trace_capacity]
+
+end share
+
 end WitnessGenerator
 
 end Clap
